src/asn1/ASN1.Spec.TLV.fst
@@ -8,18 +8,20 @@ include LowParse.Bytes
 include LowParse.Spec.DER
 include LowParse.Spec.SeqBytes.Base
 module U32 = FStar.UInt32
+
 /// Generic ASN.1 DER (Primitive) TLV Parser
 /// NOTE: For each Tag-Length-Value tuple, we firstly parse the
 ///       (Tag, Length) pair as the `parser_tag`, then use it to
 ///       choose a proper Value parser to parse the value.
 
+
 /// Parser filter for valid ASN.1 DER `Tag`, `Length` pair
 let filter_TL
   (x: asn1_type * bounded_int32 asn1_length_min asn1_length_max)
 : bool
-= let a, l = x in
+= let a, len = x in
   let min, max = bound_of_asn1_type a in
-  asn1_length_inbound (U32.v l) min max
+  asn1_length_inbound (U32.v len) min max
 
 let valid_asn1_TL = parse_filter_refine filter_TL
 
@@ -39,24 +41,24 @@ let parse_TL_unfold
   match parse parse_asn1_tag input with
   | None -> res == None
   | Some (a, consumed_a) ->
-    (let input_l = Seq.slice input consumed_a (Seq.length input) in
-     match parse (parse_bounded_der_length32 asn1_length_min asn1_length_max) input_l with
+    (let input_len = Seq.slice input consumed_a (Seq.length input) in
+     match parse (parse_bounded_der_length32 asn1_length_min asn1_length_max) input_len with
      | None -> res == None
-     | Some (l, consumed_l) ->
-       (if filter_TL (a, l) then
-        ( res == Some ((a, l), consumed_a + consumed_l) )
+     | Some (len, consumed_len) ->
+       (if filter_TL (a, len) then
+        ( res == Some ((a, len), consumed_a + consumed_len) )
         else
         ( res == None ))))
 = nondep_then_eq
   (* p1 *) (parse_asn1_tag)
   (* p2 *) (parse_bounded_der_length32 asn1_length_min asn1_length_max)
-  (* in *) input;
+  (* in *) (input);
   parse_filter_eq
   (* p  *) (parse_asn1_tag
            `nondep_then`
             parse_bounded_der_length32 asn1_length_min asn1_length_max)
   (* f  *) (filter_TL)
-  (* in *) input
+  (* in *) (input)
 
 /// Serializer for valid ASN.1 DER `Tag`, `Length` pair
 ///
@@ -72,10 +74,10 @@ let serialize_TL_unfold
   (x: parse_filter_refine filter_TL)
 : Lemma (
   let sx = serialize serialize_TL x in
-  let a, l = x in
+  let a, len = x in
   sx == (serialize (serialize_asn1_tag ()) a)
         `Seq.append`
-        (serialize (serialize_bounded_der_length32 asn1_length_min asn1_length_max) l))
+        (serialize (serialize_bounded_der_length32 asn1_length_min asn1_length_max) len))
 = serialize_nondep_then_eq
   (* s1 *) (serialize_asn1_tag ())
   (* s2 *) (serialize_bounded_der_length32 asn1_length_min asn1_length_max)
@@ -87,21 +89,70 @@ let serialize_TL_unfold
 ///
 let parser_tag_of_asn1_value
   (v: asn1_value)
-: (parse_filter_refine filter_TL)
+: Tot (parse_filter_refine filter_TL)
 = match v with
-  | BOOLEAN_VALUE      b -> (BOOLEAN     , 1ul)
-  | NULL_VALUE        () -> (NULL        , 0ul)
-  | OCTET_STRING_VALUE s -> (OCTET_STRING, U32.uint_to_t (Seq.length s))
+  | BOOLEAN_VALUE      b   -> (BOOLEAN     , 1ul)
+  | NULL_VALUE        ()   -> (NULL        , 0ul)
+  | OCTET_STRING_VALUE l s -> (OCTET_STRING, U32.uint_to_t l)
+
+// let parser_tag_of_asn1_value_impl
+//   (v: asn1_value)
+// : Tot (x: parse_filter_refine filter_TL{x == parser_tag_of_asn1_value v})
+// = match v with
+//   | BOOLEAN_VALUE      b   -> (BOOLEAN     , 1ul)
+//   | NULL_VALUE        ()   -> (NULL        , 0ul)
+//   | OCTET_STRING_VALUE l s -> (OCTET_STRING, U32.uint_to_t l)
 
 let asn1_value_of_TL = refine_with_tag parser_tag_of_asn1_value
+
+/// Synth functions
+let synth_asn1_boolean_value
+  (x: parse_filter_refine filter_TL{x == (BOOLEAN, 1ul)})
+  (b: bool)
+: refine_with_tag parser_tag_of_asn1_value x
+= BOOLEAN_VALUE b
+
+let synth_asn1_boolean_value_inverse
+  (x: parse_filter_refine filter_TL{x == (BOOLEAN, 1ul)})
+  (value: refine_with_tag parser_tag_of_asn1_value x)
+: bool
+= BOOLEAN_VALUE?.b value
+
+let synth_asn1_null_value
+  (x: parse_filter_refine filter_TL{x == (NULL, 0ul)})
+  (n: unit)
+: refine_with_tag parser_tag_of_asn1_value x
+= NULL_VALUE n
+
+let synth_asn1_null_value_inverse
+  (x: parse_filter_refine filter_TL{x == (NULL, 0ul)})
+  (value: refine_with_tag parser_tag_of_asn1_value x)
+: unit
+= NULL_VALUE?.n value
+
+let lbytes = Seq.Properties.lseq byte
+
+let synth_asn1_octet_string_value
+  (l: asn1_length_t)
+  (x: parse_filter_refine filter_TL{x == (OCTET_STRING, U32.uint_to_t l)})
+  (s: lbytes l)
+: refine_with_tag parser_tag_of_asn1_value x
+= OCTET_STRING_VALUE l s
+
+let synth_asn1_octet_string_value_inverse
+  (l: asn1_length_t)
+  (x: parse_filter_refine filter_TL{x == (OCTET_STRING, U32.uint_to_t l)})
+  (value: refine_with_tag parser_tag_of_asn1_value x)
+: (s: lbytes l)
+= OCTET_STRING_VALUE?.s value
 
 /// Strong parser kind for ASN.1 DER `Value` parser
 let parse_asn1_value_kind
   (x: parse_filter_refine filter_TL)
 : parser_kind
-= let a, l = x in
-  let len = U32.v l in
-  strong_parser_kind len len None
+= let a, len = x in
+  let l = U32.v len in
+  strong_parser_kind l l None
 
 /// Weak Strong parser kind for ASN.1 DER `Value` parser, throw "runtime" tag, length
 let parse_asn1_value_kind_weak = strong_parser_kind asn1_length_min asn1_length_max None
@@ -111,72 +162,79 @@ let parse_asn1_value_kind_weak = strong_parser_kind asn1_length_min asn1_length_
 let parse_asn1_value
   (x: parse_filter_refine filter_TL)
 : Tot (parser (parse_asn1_value_kind x) (refine_with_tag parser_tag_of_asn1_value x))
-= let a, l = x in
-  let len = U32.v l in
+= let a, len = x in
+  let l: asn1_length_t = U32.v len in
   match a with
   | BOOLEAN      -> (parse_asn1_value_kind x
                      `weaken`
                     (parse_asn1_boolean
                      `parse_synth`
-                    (fun b -> BOOLEAN_VALUE b <: refine_with_tag parser_tag_of_asn1_value x)))
+                    // (fun b -> BOOLEAN_VALUE b <: refine_with_tag parser_tag_of_asn1_value x)
+                    (synth_asn1_boolean_value x)))
 
   | NULL         -> (parse_asn1_value_kind x
                      `weaken`
                     (parse_asn1_null
                      `parse_synth`
-                    (fun n -> NULL_VALUE n <: refine_with_tag parser_tag_of_asn1_value x)))
+                    // (fun n -> NULL_VALUE n <: refine_with_tag parser_tag_of_asn1_value x)
+                    (synth_asn1_null_value x)))
 
   | OCTET_STRING -> (parse_asn1_value_kind x
                      `weaken`
-                    (parse_seq_flbytes len
+                    (parse_seq_flbytes l
                      `parse_synth`
-                    (fun s -> OCTET_STRING_VALUE s <: refine_with_tag parser_tag_of_asn1_value x)))
+                    // (fun (s: lbytes len) -> OCTET_STRING_VALUE s len <: refine_with_tag parser_tag_of_asn1_value x)
+                    (synth_asn1_octet_string_value l x)))
 
+// #push-options "--query_stats --z3rlimit 32 --max_fuel 16 --max_ifuel 16"
 let parse_asn1_value_unfold
   (x: parse_filter_refine filter_TL)
   (input: bytes)
 : Lemma (
-  let a, l = x in
-  let len = U32.v l in
+  let a, len = x in
+  let l: asn1_length_t = U32.v len in
   let value = parse (parse_asn1_value x) input in
   match a with
   | BOOLEAN      -> (match parse parse_asn1_boolean input with
                      | None -> value == None
                      | Some (b, consumed) ->
                             parser_tag_of_asn1_value (BOOLEAN_VALUE b) == x /\
-                            consumed == len /\
+                            consumed == l /\
                             value == Some (BOOLEAN_VALUE b, consumed))
 
   | NULL         -> (match parse parse_asn1_null input with
                      | None -> value == None
                      | Some (null, consumed) ->
                             parser_tag_of_asn1_value (NULL_VALUE null) == x /\
-                            consumed == len /\
+                            consumed == l /\
                             value == Some (NULL_VALUE null, consumed))
 
-  | OCTET_STRING -> (match parse (parse_seq_flbytes len) input with
+  | OCTET_STRING -> (match parse (parse_seq_flbytes l) input with
                      | None -> value == None
-                     | Some (s, consumed) ->
-                            parser_tag_of_asn1_value (OCTET_STRING_VALUE s) == x /\
-                            consumed == len /\
-                            value == Some (OCTET_STRING_VALUE s, consumed)))
-= let a, l = x in
-  let len = U32.v l in
+                     | Some (s, consumed) -> True \/
+                            parser_tag_of_asn1_value (OCTET_STRING_VALUE l s) == x /\
+                            consumed == l /\
+                            value == Some (OCTET_STRING_VALUE l s, consumed)))
+= let a, len = x in
+  let l = U32.v len in
   match a with
   | BOOLEAN      -> (parse_asn1_boolean_unfold input;
                      parse_synth_eq
                      (* p1 *) (parse_asn1_boolean)
-                     (* f2 *) (fun b -> BOOLEAN_VALUE b <: refine_with_tag parser_tag_of_asn1_value x)
+                     (* f2 *) (synth_asn1_boolean_value x)
+                           // (fun b -> BOOLEAN_VALUE b <: refine_with_tag parser_tag_of_asn1_value x)
                      (* in *) input)
 
   | NULL         -> (parse_synth_eq
                      (* p1 *) (parse_asn1_null)
-                     (* f2 *) (fun n -> NULL_VALUE n <: refine_with_tag parser_tag_of_asn1_value x)
+                     (* f2 *) (synth_asn1_null_value x)
+                           // (fun n -> NULL_VALUE n <: refine_with_tag parser_tag_of_asn1_value x)
                      (* in *) input)
 
   | OCTET_STRING -> (parse_synth_eq
-                     (* p1 *) (parse_seq_flbytes len)
-                     (* f2 *) (fun s -> OCTET_STRING_VALUE s <: refine_with_tag parser_tag_of_asn1_value x)
+                     (* p1 *) (parse_seq_flbytes l)
+                     (* f2 *) (synth_asn1_octet_string_value l x)
+                           // (fun (s: lbytes len) -> OCTET_STRING_VALUE s len <: refine_with_tag parser_tag_of_asn1_value x)
                      (* in *) input)
 
 /// Serializer for ASN.1 DER `Value`
@@ -184,77 +242,84 @@ let parse_asn1_value_unfold
 let serialize_asn1_value
   (x: parse_filter_refine filter_TL)
 : Tot (serializer (parse_asn1_value x))
-= let a, l = x in
-  let len = U32.v l in
+= let a, len = x in
+  let l = U32.v len in
   match a with
   | BOOLEAN      -> (parse_asn1_value_kind x
                     `serialize_weaken`
                     (serialize_synth
                      (* p1 *) (parse_asn1_boolean)
-                     (* f2 *) (fun b -> BOOLEAN_VALUE b <: refine_with_tag parser_tag_of_asn1_value x)
+                     (* f2 *) (synth_asn1_boolean_value x)
+                           // (fun b -> BOOLEAN_VALUE b <: refine_with_tag parser_tag_of_asn1_value x)
                      (* s1 *) (serialize_asn1_boolean)
-                     (* g1 *) (fun v -> BOOLEAN_VALUE?.b v)
+                     (* g1 *) (synth_asn1_boolean_value_inverse x)
+                           // (fun v -> BOOLEAN_VALUE?.b v)
                      (* prf*) ()))
 
   | NULL         -> (parse_asn1_value_kind x
                      `serialize_weaken`
                     (serialize_synth
                      (* p1 *) (parse_asn1_null)
-                     (* f2 *) (fun n -> NULL_VALUE n <: refine_with_tag parser_tag_of_asn1_value x)
+                     (* f2 *) (synth_asn1_null_value x)
+                           // (fun n -> NULL_VALUE n <: refine_with_tag parser_tag_of_asn1_value x)
                      (* s1 *) (serialize_asn1_null)
-                     (* g1 *) (fun v -> NULL_VALUE?.n v)
+                     (* g1 *) (synth_asn1_null_value_inverse x)
+                           // (fun v -> NULL_VALUE?.n v)
                      (* prf*) ()))
 
   | OCTET_STRING -> (parse_asn1_value_kind x
                      `serialize_weaken`
                     (serialize_synth
-                     (* p1 *) (parse_seq_flbytes len)
-                     (* f2 *) (fun s -> OCTET_STRING_VALUE s <: refine_with_tag parser_tag_of_asn1_value x)
-                     (* s1 *) (serialize_seq_flbytes len)
-                     (* g1 *) (fun v -> OCTET_STRING_VALUE?.s v)
+                     (* p1 *) (parse_seq_flbytes l)
+                     (* f2 *) (synth_asn1_octet_string_value l x)
+                     (* s1 *) (serialize_seq_flbytes l)
+                     (* g1 *) (synth_asn1_octet_string_value_inverse l x)
                      (* prf*) ()))
 
 let serialize_asn1_value_unfold
   (x: parse_filter_refine filter_TL)
   (value: refine_with_tag parser_tag_of_asn1_value x)
 : Lemma (
-  let a, l = x in
-  let len = U32.v l in
+  let a, len = x in
+  let l = U32.v len in
   let sx = serialize (serialize_asn1_value x) value in
   match a with
   | BOOLEAN      -> (sx == serialize serialize_asn1_boolean      (BOOLEAN_VALUE?.b value)      /\
-                     len == Seq.length sx)
+                     l == Seq.length sx)
   | NULL         -> (sx == serialize serialize_asn1_null         (NULL_VALUE?.n value)         /\
-                     len == Seq.length sx)
-  | OCTET_STRING -> (sx == serialize (serialize_seq_flbytes len) (OCTET_STRING_VALUE?.s value) /\
-                     len == Seq.length sx))
-= let a, l = x in
-  let len = U32.v l in
+                     l == Seq.length sx)
+  | OCTET_STRING -> (sx == serialize (serialize_seq_flbytes l) (OCTET_STRING_VALUE?.s value) /\
+                     l == Seq.length sx))
+= let a, len = x in
+  let l = U32.v len in
   match a with
   | BOOLEAN      -> (serialize_synth_eq
                      (* p1 *) (parse_asn1_boolean)
-                     (* f2 *) (fun b -> BOOLEAN_VALUE b <: refine_with_tag parser_tag_of_asn1_value x)
+                     (* f2 *) (synth_asn1_boolean_value x)
+                           // (fun b -> BOOLEAN_VALUE b <: refine_with_tag parser_tag_of_asn1_value x)
                      (* s1 *) (serialize_asn1_boolean)
-                     (* g1 *) (fun v -> BOOLEAN_VALUE?.b v)
+                     (* g1 *) (synth_asn1_boolean_value_inverse x)
+                           // (fun v -> BOOLEAN_VALUE?.b v)
                      (* prf*) ()
-                     (* x  *) value)
+                     (* x  *) (value))
 
   | NULL         -> (serialize_synth_eq
                      (* p1 *) (parse_asn1_null)
-                     (* f2 *) (fun n -> NULL_VALUE n <: refine_with_tag parser_tag_of_asn1_value x)
+                     (* f2 *) (synth_asn1_null_value x)
+                           // (fun n -> NULL_VALUE n <: refine_with_tag parser_tag_of_asn1_value x)
                      (* s1 *) (serialize_asn1_null)
-                     (* g1 *) (fun v -> NULL_VALUE?.n v)
+                     (* g1 *) (synth_asn1_null_value_inverse x)
+                           // (fun v -> NULL_VALUE?.n v)
                      (* prf*) ()
-                     (* x  *) value)
+                     (* x  *) (value))
 
   | OCTET_STRING -> (serialize_synth_eq
-                     (* p1 *) (parse_seq_flbytes len)
-                     (* f2 *) (fun s -> OCTET_STRING_VALUE s <: refine_with_tag parser_tag_of_asn1_value x)
-                     (* s1 *) (serialize_seq_flbytes len)
-                     (* g1 *) (fun v -> OCTET_STRING_VALUE?.s v)
+                     (* p1 *) (parse_seq_flbytes l)
+                     (* f2 *) (synth_asn1_octet_string_value l x)
+                     (* s1 *) (serialize_seq_flbytes l)
+                     (* g1 *) (synth_asn1_octet_string_value_inverse l x)
                      (* prf*) ()
-                     (* x  *) value)
-
+                     (* x  *) (value))
 
 
 /// Kind for ASN.1 DER Tag, Length, Value tuple parser
